add step-indexing to local sim

theories/sim/local.v
@@ -11,28 +11,29 @@ Variable (wsat: A → state → state → Prop).
 Variable (vrel: A → expr → expr → Prop).
 Variable (fns fnt: fn_env).
 
-(* TODO: encode what it means for the context to not contain our private tags! *)
-(* TODO: how do we know we're at the top of the stack? *)
 Inductive _sim_local_body
-  (sim_local_body : A → expr → state → expr → state → Prop)
-  (r: A) : expr → state → expr → state → Prop :=
+  (sim_local_body : A → nat → expr → state → expr → state → Prop)
+  (r: A) (idx: nat) : expr → state → expr → state → Prop :=
 (* If src is stuck, then anything is related *)
 | sim_local_body_stuck e_src σ_src e_tgt σ_tgt
     (STUCK: stuck (Λ:=bor_lang fns) e_src σ_src)
-    : _sim_local_body sim_local_body r e_src σ_src e_tgt σ_tgt
+    : _sim_local_body sim_local_body r idx e_src σ_src e_tgt σ_tgt
 (* If tgt makes 1 step, src can make some step *)
 | sim_local_body_step e_src σ_src e_tgt σ_tgt
     (STEP: ∀ r_f e_tgt' σ_tgt'
-      (* for any frame r_f that is compatible with our resource r and has world satisfaction *)
-      (VALID: ✓ (r_f ⋅ r)) (WSAT: wsat (r_f ⋅ r) σ_src σ_tgt)
+      (* for any frame r_f that is compatible with our resource r *)
+      (VALID: ✓ (r_f ⋅ r))
+      (* and has world satisfaction *)
+      (WSAT: wsat (r_f ⋅ r) σ_src σ_tgt)
       (* if tgt can locally make 1 step *)
       (STEPT: (e_tgt, σ_tgt) ~{fnt}~> (e_tgt', σ_tgt')),
       (* then we locally can makes some step and pick a new resource r' *)
-      ∃ e_src' σ_src' r',
-        (e_src, σ_src) ~{fns}~>* (e_src', σ_src') ∧
+      ∃ e_src' σ_src' r' idx',
+        ((e_src, σ_src) ~{fns}~>+ (e_src', σ_src') ∨
+         ((idx' < idx)%nat ∧ (e_src', σ_src') = (e_src, σ_src))) ∧
         ✓ (r_f ⋅ r') ∧ wsat (r_f ⋅ r') σ_src' σ_tgt' ∧
-        sim_local_body r' e_src' σ_src' e_tgt' σ_tgt')
-    : _sim_local_body sim_local_body r e_src σ_src e_tgt σ_tgt
+        sim_local_body r' idx' e_src' σ_src' e_tgt' σ_tgt')
+    : _sim_local_body sim_local_body r idx e_src σ_src e_tgt σ_tgt
 (* If tgt prepares to make a call to [name], src should be able to make the same
   call. Here we do not want to step into the call of [name], but to step over it. *)
 | sim_local_body_step_over_call
@@ -41,14 +42,16 @@ Inductive _sim_local_body
     fid e_src e_tgt el_tgt σ_src σ_tgt
     (CALLTGT: e_tgt = fill K_tgt (Call #[ScFnPtr fid] el_tgt))
     (STEPOVER: ∀ r_f
-        (* for any frame r_f that is compatible with our resource r and has world satisfaction *)
+        (* for any frame r_f that is compatible with our resource r *)
         (VALID: ✓ (r_f ⋅ r))
+        (* and has world satisfaction *)
         (WSAT : wsat (r_f ⋅ r) σ_src σ_tgt)
         (* tgt is ready to make a call of [name] *)
         (VTGT : Forall (λ ei, is_Some (to_value ei)) el_tgt),
         (* then src is also ready to make a call of [name] *)
         ∃ el_src σ1_src rc rv,
-        (e_src, σ_src) ~{fns}~>* (fill K_src (Call #[ScFnPtr fid] el_src), σ1_src) ∧
+        (e_src, σ_src) ~{fns}~>*
+          (fill K_src (Call #[ScFnPtr fid] el_src), σ1_src) ∧
         Forall (λ ei, is_Some (to_value ei)) el_src ∧
         (* and we can pick a resource [rv] for the arguments *)
         ✓ (r_f ⋅ (rc ⋅ rv)) ∧ wsat (r_f ⋅ (rc ⋅ rv)) σ1_src σ_tgt ∧
@@ -57,15 +60,15 @@ Inductive _sim_local_body
         (* and after the call our context can continue *)
         (∀ r_f' r' v_src v_tgt σ_src' σ_tgt'
           (* For any new resource r' and frame r_f' that are compatible with
-             our local resource r and has world satisfaction *)
+             our local resource r and have world satisfaction *)
           (VALID': ✓ (r_f' ⋅ (rc ⋅ r')))
           (WSAT' : wsat (r_f ⋅ (rc ⋅ r')) σ_src' σ_tgt')
           (* and the returned values are related w.r.t. (r ⋅ r' ⋅ r_f) *)
           (VRET  : vrel r' (Val v_src) (Val v_tgt)),
-          sim_local_body (rc ⋅ r')
-                      (fill K_src (Val v_src)) σ_src'
-                      (fill K_tgt (Val v_tgt)) σ_tgt'))
-    : _sim_local_body sim_local_body r e_src σ_src e_tgt σ_tgt
+          ∃ idx', sim_local_body (rc ⋅ r') idx'
+                                  (fill K_src (Val v_src)) σ_src'
+                                  (fill K_tgt (Val v_tgt)) σ_tgt'))
+    : _sim_local_body sim_local_body r idx e_src σ_src e_tgt σ_tgt
 (* If tgt prepares to end, src also prepares to end *)
 | sim_local_body_end_call v_src σ_src v_tgt σ_tgt e_src e_tgt
     (ESRC: e_src = EndCall (Val v_src))
@@ -82,25 +85,25 @@ Inductive _sim_local_body
         ✓ (r_f ⋅ r') ∧ wsat (r_f ⋅ r') eσ_src'.2 eσ_tgt'.2 ∧
         (* and the returned values are related *)
         vrel r' (Val v_src) (Val v_tgt))
-    : _sim_local_body sim_local_body r e_src σ_src e_tgt σ_tgt
+    : _sim_local_body sim_local_body r idx e_src σ_src e_tgt σ_tgt
 .
 
-Lemma sim_local_body_mono : monotone5 _sim_local_body.
+Lemma sim_local_body_mono : monotone6 _sim_local_body.
 Proof.
-  intros r es σs et σt R R' SIM LE; inversion SIM; subst.
+  intros r idx es σs et σt R R' SIM LE; inversion SIM; subst.
   - by eapply sim_local_body_stuck; eauto.
   - eapply sim_local_body_step. naive_solver.
   - eapply sim_local_body_step_over_call; eauto. naive_solver.
   - by eapply sim_local_body_end_call; eauto.
 Qed.
 
-Definition sim_local_body := paco5 _sim_local_body bot5.
+Definition sim_local_body := paco6 _sim_local_body bot6.
 
 Lemma sim_local_body_resource_mono r1 r2
   (SAT_DOWNWARD: ∀ r1 r2, r1 ≼ r2 → wsat r2 <2= wsat r1) :
-  r1 ≼ r2 → sim_local_body r1 <4= sim_local_body r2.
+  r1 ≼ r2 → sim_local_body r1 <5= sim_local_body r2.
 Proof.
-  revert r1 r2. pcofix CIH. intros r1 r2 LE es σs et σt SIM.
+  revert r1 r2. pcofix CIH. intros r1 r2 LE idx es σs et σt SIM.
   pfold. punfold SIM; [|apply sim_local_body_mono].
   inversion SIM; subst.
   - by eapply sim_local_body_stuck.
@@ -110,8 +113,9 @@ Proof.
     { eapply cmra_valid_included; [exact VL2|by apply cmra_mono_l]. }
     have WS1: wsat (r_f ⋅ r1) σs σt.
     { eapply SAT_DOWNWARD; [by apply cmra_mono_l|exact WS2]. }
-    destruct (STEP _ _ _ VL1 WS1 STEPT) as (es' & cs' & r' & STEPS' & VL' & WS' & SIM').
-    exists es', cs', r'. do 3 (split; [done|]).
+    destruct (STEP _ _ _ VL1 WS1 STEPT) as
+      (es' & cs' & r' & idx' & STEPS' & VL' & WS' & SIM').
+    exists es', cs', r', idx'. do 3 (split; [done|]).
     right. eapply CIH; eauto. by inversion SIM'.
   - eapply sim_local_body_step_over_call; eauto.
     intros r_f VL2 WS2 FAT.
@@ -123,8 +127,8 @@ Proof.
       as (es' & cs & rc & rv & STEPS & FAS & VL & WS & VREL & HK).
     exists es', cs, rc, rv. do 5 (split; [done|]).
     intros r_f' r' vs vt cs' ct' VL' WS' VREL'.
-    specialize (HK _ _ _ _ _ _ VL' WS' VREL').
-    right. eapply CIH; [eauto|by inversion HK].
+    destruct (HK _ _ _ _ _ _ VL' WS' VREL') as [idx' HK2].
+    exists idx'. right. eapply CIH; [eauto|by inversion HK2].
   - eapply sim_local_body_end_call; [eauto..|].
     intros r_f ct' VL2 WS2 STEPT.
     have VL1: ✓ (r_f ⋅ r1).
@@ -146,7 +150,7 @@ Definition sim_local_fun (fn_src fn_tgt : function) : Prop :=
     (EQT: match fn_tgt with
           | FunV xl e => subst_l xl el_tgt e = Some e_tgt
           end),
-    sim_local_body r (InitCall e_src) σ_src (InitCall e_tgt) σ_tgt.
+    ∃ idx, sim_local_body r idx (InitCall e_src) σ_src (InitCall e_tgt) σ_tgt.
 
 Definition sim_local_funs : Prop :=
   ∀ name fn_src, fns !! name = Some fn_src → ∃ fn_tgt,
@@ -167,7 +171,8 @@ Variable (vrel: A → expr → expr → Prop).
 Record sim_prog (prog_src prog_tgt: fn_env) := {
   sim_prog_env: sim_local_funs wsat vrel prog_src prog_tgt;
   sim_prog_main:
-    sim_local_body wsat vrel prog_src prog_tgt ε
-                   (Call #["main"] []) init_state (Call #["main"] []) init_state;
+    ∃ idx, sim_local_body wsat vrel prog_src prog_tgt ε idx
+                          (Call #["main"] []) init_state
+                          (Call #["main"] []) init_state;
 }.
 End program.
